<?xml version="1.0"?>


<!DOCTYPE rdf:RDF [
    <!ENTITY owl "http://www.w3.org/2002/07/owl#" >
    <!ENTITY obo "http://purl.obolibrary.org/obo/" >
    <!ENTITY owl2 "http://www.w3.org/2006/12/owl2#" >
    <!ENTITY xsd "http://www.w3.org/2001/XMLSchema#" >
    <!ENTITY owl2xml "http://www.w3.org/2006/12/owl2-xml#" >
    <!ENTITY rdfs "http://www.w3.org/2000/01/rdf-schema#" >
    <!ENTITY rdf "http://www.w3.org/1999/02/22-rdf-syntax-ns#" >
]>


<rdf:RDF xmlns="http://purl.obolibrary.org/obo/vo/external/ro_proposed_import.owl#"
     xml:base="http://purl.obolibrary.org/obo/vo/external/ro_proposed_import.owl"
     xmlns:obo="http://purl.obolibrary.org/obo/"
     xmlns:rdfs="http://www.w3.org/2000/01/rdf-schema#"
     xmlns:owl2xml="http://www.w3.org/2006/12/owl2-xml#"
     xmlns:owl="http://www.w3.org/2002/07/owl#"
     xmlns:xsd="http://www.w3.org/2001/XMLSchema#"
     xmlns:rdf="http://www.w3.org/1999/02/22-rdf-syntax-ns#"
     xmlns:owl2="http://www.w3.org/2006/12/owl2#">
    <owl:Ontology rdf:about="http://purl.obolibrary.org/obo/vo/external/ro_proposed_import.owl"/>
    


    <!-- 
    ///////////////////////////////////////////////////////////////////////////////////////
    //
    // Annotation properties
    //
    ///////////////////////////////////////////////////////////////////////////////////////
     -->

    <owl:AnnotationProperty rdf:about="http://purl.obolibrary.org/obo/IAO_0000115"/>
    <owl:AnnotationProperty rdf:about="http://purl.obolibrary.org/obo/IAO_0000412"/>
    <owl:AnnotationProperty rdf:about="http://purl.obolibrary.org/obo/IAO_0000111"/>
    


    <!-- 
    ///////////////////////////////////////////////////////////////////////////////////////
    //
    // Datatypes
    //
    ///////////////////////////////////////////////////////////////////////////////////////
     -->

    


    <!-- 
    ///////////////////////////////////////////////////////////////////////////////////////
    //
    // Object Properties
    //
    ///////////////////////////////////////////////////////////////////////////////////////
     -->

    


    <!-- http://purl.obolibrary.org/obo/activates -->

    <owl:ObjectProperty rdf:about="http://purl.obolibrary.org/obo/activates">
        <rdfs:label xml:lang="en">activates</rdfs:label>
        <obo:IAO_0000412 rdf:datatype="http://www.w3.org/2001/XMLSchema#anyURI">http://purl.org/obo/owl/ro_proposed</obo:IAO_0000412>
        <obo:IAO_0000111 xml:lang="en">activates</obo:IAO_0000111>
        <rdfs:subPropertyOf rdf:resource="http://purl.obolibrary.org/obo/positively_regulates"/>
    </owl:ObjectProperty>
    


    <!-- http://purl.obolibrary.org/obo/bearer_of -->

    <owl:ObjectProperty rdf:about="http://purl.obolibrary.org/obo/bearer_of">
        <rdfs:label xml:lang="en">bearer_of</rdfs:label>
        <obo:IAO_0000412 rdf:datatype="http://www.w3.org/2001/XMLSchema#anyURI">http://purl.org/obo/owl/ro_proposed</obo:IAO_0000412>
        <obo:IAO_0000115 xml:lang="en">A relation between an entity and a dependent continuant; the reciprocal relation of inheres_in</obo:IAO_0000115>
        <obo:IAO_0000111 xml:lang="en">bearer_of</obo:IAO_0000111>
    </owl:ObjectProperty>
    


    <!-- http://purl.obolibrary.org/obo/inheres_in -->

    <owl:ObjectProperty rdf:about="http://purl.obolibrary.org/obo/inheres_in">
        <rdfs:label xml:lang="en">inheres_in</rdfs:label>
        <obo:IAO_0000412 rdf:datatype="http://www.w3.org/2001/XMLSchema#anyURI">http://purl.org/obo/owl/ro_proposed</obo:IAO_0000412>
        <obo:IAO_0000115 xml:lang="en">A relation between a dependent continuant D and an entity E. D inheres_in E iff: given any d that instantiates D at t, there exists some e that instantiates E at t and d *inheres_in* e at t. Here *inheres_in* is the primitive instance level relation.</obo:IAO_0000115>
        <obo:IAO_0000111 xml:lang="en">inheres_in</obo:IAO_0000111>
        <rdfs:subPropertyOf rdf:resource="http://purl.obolibrary.org/obo/inheres_in_part_of"/>
    </owl:ObjectProperty>
    


    <!-- http://purl.obolibrary.org/obo/inheres_in_part_of -->

    <owl:ObjectProperty rdf:about="http://purl.obolibrary.org/obo/inheres_in_part_of">
        <rdfs:label xml:lang="en">inheres_in_part_of</rdfs:label>
        <obo:IAO_0000412 rdf:datatype="http://www.w3.org/2001/XMLSchema#anyURI">http://purl.org/obo/owl/ro_proposed</obo:IAO_0000412>
        <obo:IAO_0000111 xml:lang="en">inheres_in_part_of</obo:IAO_0000111>
    </owl:ObjectProperty>
    


    <!-- http://purl.obolibrary.org/obo/positively_regulates -->

    <owl:ObjectProperty rdf:about="http://purl.obolibrary.org/obo/positively_regulates">
        <rdfs:label xml:lang="en">positively_regulates</rdfs:label>
        <obo:IAO_0000412 rdf:datatype="http://www.w3.org/2001/XMLSchema#anyURI">http://purl.org/obo/owl/ro_proposed</obo:IAO_0000412>
        <obo:IAO_0000115 xml:lang="en">A regulation relation in which the unfolding of the regulating process *increases* the frequency, rate or extent of the regulated process</obo:IAO_0000115>
        <obo:IAO_0000111 xml:lang="en">positively_regulates</obo:IAO_0000111>
        <rdfs:subPropertyOf rdf:resource="http://purl.obolibrary.org/obo/regulates"/>
    </owl:ObjectProperty>
    


    <!-- http://purl.obolibrary.org/obo/regulates -->

    <owl:ObjectProperty rdf:about="http://purl.obolibrary.org/obo/regulates">
        <rdfs:label xml:lang="en">regulates</rdfs:label>
        <obo:IAO_0000412 rdf:datatype="http://www.w3.org/2001/XMLSchema#anyURI">http://purl.org/obo/owl/ro_proposed</obo:IAO_0000412>
        <obo:IAO_0000115 xml:lang="en">A relation between a process and a process or quality. A regulates B if the unfolding of A affects the frequency, rate or extent of B. A is called the regulating process, B the regulates process</obo:IAO_0000115>
        <obo:IAO_0000111 xml:lang="en">regulates</obo:IAO_0000111>
    </owl:ObjectProperty>
    


    <!-- http://purl.obolibrary.org/obo/role_of -->

    <owl:ObjectProperty rdf:about="http://purl.obolibrary.org/obo/role_of">
        <rdfs:label xml:lang="en">role_of</rdfs:label>
        <obo:IAO_0000412 rdf:datatype="http://www.w3.org/2001/XMLSchema#anyURI">http://purl.org/obo/owl/ro_proposed</obo:IAO_0000412>
        <obo:IAO_0000115 xml:lang="en">A relation between a role R and an entity E. R role_of E iff: R inheres_in E and R is a role</obo:IAO_0000115>
        <obo:IAO_0000111 xml:lang="en">role_of</obo:IAO_0000111>
        <rdfs:subPropertyOf rdf:resource="http://purl.obolibrary.org/obo/inheres_in"/>
    </owl:ObjectProperty>
    


    <!-- http://purl.obolibrary.org/obo/stimulates -->

    <owl:ObjectProperty rdf:about="http://purl.obolibrary.org/obo/stimulates">
        <rdfs:label xml:lang="en">stimulates</rdfs:label>
        <obo:IAO_0000412 rdf:datatype="http://www.w3.org/2001/XMLSchema#anyURI">http://purl.org/obo/owl/ro_proposed</obo:IAO_0000412>
        <obo:IAO_0000111 xml:lang="en">stimulates</obo:IAO_0000111>
    </owl:ObjectProperty>
    


    <!-- http://purl.obolibrary.org/obo/unfolds_in -->

    <owl:ObjectProperty rdf:about="http://purl.obolibrary.org/obo/unfolds_in">
        <rdfs:label xml:lang="en">unfolds_in</rdfs:label>
        <obo:IAO_0000412 rdf:datatype="http://www.w3.org/2001/XMLSchema#anyURI">http://purl.org/obo/owl/ro_proposed</obo:IAO_0000412>
        <obo:IAO_0000115 xml:lang="en">P unfolds_in C : the execution of P is spatially contained by C. forall pP,  forall c&#39; partipates_in p, c&#39; located_in C at t, for some t in P</obo:IAO_0000115>
        <obo:IAO_0000111 xml:lang="en">unfolds_in</obo:IAO_0000111>
    </owl:ObjectProperty>
</rdf:RDF>



<!-- Generated by the OWL API (version 3.2.2.1782) http://owlapi.sourceforge.net -->